theories/base.v
@@ -31,6 +31,8 @@ Hint Unfold cast : deriving.
 Notation "e1 * e2" := (etrans e1 e2) : deriving_scope.
 Notation "e ^-1" := (esym e) : deriving_scope.
 
+Hint Unfold etrans esym Logic.eq_sym Logic.eq_trans : deriving.
+
 (* We redefine some constants of the standard library here to avoid problems
    with universe inconsistency and opacity. *)
 
@@ -173,6 +175,8 @@ Hint Unfold map : deriving.
 Hint Unfold foldr : deriving.
 Hint Unfold sumn : deriving.
 Hint Unfold cat : deriving.
+Hint Unfold flatten : deriving.
+Hint Unfold all : deriving.
 
 Fixpoint fin n :=
   if n is n.+1 then option (fin n) else void.
@@ -1169,3 +1173,60 @@ Definition hnth1V m :=
   end.
 Coercion hnth1V : hlist1V >-> Funclass.
 Hint Unfold hnth1V : deriving.
+
+Section LiftClass.
+
+Import PolyType.
+
+Variables (K : Type) (sort : K -> Type).
+
+Definition eq_class X := {sX : K | sort sX = X}.
+
+Record tagged_sort n := TaggedSort {
+  untag_sort :> fin n -> Type;
+}.
+
+Definition ts_nil_tag n Ts := @TaggedSort n Ts.
+Canonical ts_cons_tag n Ts := @ts_nil_tag n Ts.
+
+Record lift_class n := LiftClass {
+  lift_class_sort  :> tagged_sort n;
+  _ :  forall i, eq_class (lift_class_sort i);
+}.
+
+Definition lift_class_class n (sTs : lift_class n) :=
+  let: LiftClass _ cTs := sTs return forall i, eq_class (sTs i) in cTs.
+
+Canonical nil_lift_class f :=
+  @LiftClass 0 (ts_nil_tag f) (fun i => match i with end).
+
+Canonical cons_lift_class n
+  (sT : K) (f : lift_class n) (g : fun_split (sort sT) f) :=
+  @LiftClass n.+1 (ts_cons_tag g)
+             (fun i =>
+                match i with
+                | None   => cast eq_class (fsE1 g)   (exist _ sT erefl)
+                | Some i => cast eq_class (fsE2 g i) (lift_class_class f i)
+                end).
+
+Definition lift_class_proj n cK
+           (class : forall sT, cK (sort sT))
+           (sTs : lift_class n) (i : fin n)
+  : cK (sTs i) :=
+  cast cK (svalP (lift_class_class sTs i)) (class _).
+
+End LiftClass.
+
+Hint Unfold
+  eq_class
+  untag_sort
+  ts_nil_tag
+  ts_cons_tag
+  lift_class_sort
+  lift_class_class
+  nil_lift_class
+  cons_lift_class
+  lift_class_proj
+  : deriving.
+
+Arguments lift_class_proj {K sort n cK} class sTs i.
